lean_frontend/relsem/RelSem/PerStepSmoke.lean
@@ -27,6 +27,7 @@
 -/
 
 import RelSem.PerStepCall
+import RelSem.PerStepOwnP
 import RelSem.T1
 import RelSem.T1AppEq
 
