lean_frontend/relsem/RelSem/T1Threaded.lean
@@ -35,6 +35,7 @@
 
 import RelSem.Threaded
 import RelSem.PerStepTactics
+import RelSem.PerStepOwnP
 import RelSem.T1
 
 set_option autoImplicit false
